<b>Direct Proof of P ⇒ Q</b>
1) Assume LHS is <strong>T</strong>
2) Argue RHS is <strong>T</strong>
p → q ≡ ¬ q → ¬ p

<b>Indirect Proof (By Contrapositive)</b>
1) Assume RHS is <strong>F</strong>
2) Argue LHS is <strong>F</strong>

Therefore, both (p or q) ⊕ (p ∧ q) is <strong>T</strong> ∧ ¬ p is <strong>T</strong>. Then, P is <strong>F</strong>. Therefore, p ^ q is <strong>F</strong>. Then p or q is <strong>T</strong>. Means q is <strong>T</strong> which means q is <strong>T</strong> since p is <strong>F</strong>. So the implication is valid.

Then p ∧ r is <strong>T</strong>. Therefore both p ∧ r are <strong>T</strong>. So, p or q is <strong>T</strong> (since p is <strong>T</strong>). (p or q) ⊕ (p ∧ r) is <strong>F</strong>. So LHS is <strong>F</strong>. So the implication is valid. 

Assume LHS is <strong>T</strong>
1) p or q <strong>T</strong> ∧ (p ∧ r | <strong>F</strong>)
2) p or q | <strong>T</strong> | ∧ p ∧ r | <strong>F</strong>

Both p or r is <strong>T</strong> ∧ p ⊕ q is <strong>T</strong>. Want to show q → r is <strong>T</strong>. So assume q is <strong>T</strong>. Since p ⊕ q is <strong>T</strong>, p is <strong>F</strong>. Since p or r is <strong>T</strong>, so r is <strong>T</strong> which is what we needed to show. So RHS is <strong>T</strong>. 

>Implication is Valid

Assume RHS is <strong>F</strong>. So q → r is <strong>F</strong>. means q is <strong>T</strong> ∧ r is <strong>F</strong>. 

1)  p <strong>T</strong>: Since q is also <strong>T</strong> p ⊕ q is <strong>F</strong> then LHS is <strong>F</strong>
2) p <strong>F</strong>: Since r is also <strong>F</strong> p or is also <strong>F</strong> LHS is <strong>F</strong>
